library/cas/Cas/Schema/Codec/Laws/Mutual.lean
@@ -135,6 +135,7 @@ private theorem roundtrip_all :
         (hstruct fs (encodeFields fs x) rfl (by simpa only [encode] using hv))
     | ref t => exact False.elim (href t rfl)
     | decl _ _ _ => exact x.elim
+    | union _ _ => exact x.elim
   case case15 =>
     intro hnd hwf x hv
     cases x
